bloom-filter/src-fstar/Test.BloomFilter.fst
@@ -1,0 +1,52 @@
+module Test.BloomFilter
+
+open Rust
+open BloomFilter
+open Spec.BloomFilter
+
+module U64 = FStar.UInt64
+module Usize = FStar.UInt32
+module U32 = FStar.UInt32
+module U8 = FStar.UInt8
+module I64 = FStar.Int64
+module Isize = FStar.Int32
+module I32 = FStar.Int32
+
+
+let hash (i:usize) : All.ML u32 =
+  let hash : u32 = i in
+  let hash = U32.(hash ^^ (hash <<^ U32.uint_to_t 12)) in
+  let hash = U32.(hash ^^ (0xa5d8f52cul >>^ (i %^ 0xfful)) +%^ (hash &^ 0x589dcul)) in
+  let hash = U32.(hash -%^ (hash |^ (hash <<^ U32.uint_to_t 4))) in
+  hash
+
+let print_bool (b:bool) : All.ML unit =
+   if b then IO.print_string "true" else IO.print_string "false"
+
+let test () : All.ML unit =
+  IO.print_string "Beginning bloom filter test.\n";
+  let bf = new_bloom_filter () in
+  let bf = { bf with storage =  iter_range_ml 0ul 1000ul (fun i bf ->
+     let bf = insert_hash bf (hash i) in
+     bf
+  ) bf.storage } in
+  iter_range_ml 0ul 1000ul (fun i () ->
+    assert_eq #bool "1"
+      print_bool
+      (might_contain_hash bf.storage (hash i))
+      true
+  ) ();
+  let bf = { bf with storage = iter_range_ml 0ul 100ul (fun i bf ->
+    let bf = remove_hash bf (hash i) in
+    bf
+  ) bf.storage } in
+  iter_range_ml 100ul 1000ul (fun i () ->
+    assert_eq #bool "2"
+      print_bool
+      (might_contain_hash bf.storage (hash i))
+      true
+  ) ();
+  IO.print_string "End of test. If nothing appeared then it passed !\n"
+
+
+let _ = test ()
